# ---
# header-includes: 
#   - \usepackage{amsmath}
# ---

# Compartmental Model Solutions

$$\dot{S}=F(S,I)$$
$$\dot{I}=G(S,I)$$

$$\dot{S} = -\beta SI + \alpha R$$
$$\dot{I} = \beta SI - \gamma I$$
$$\dot{R} = \gamma I - \alpha R$$

$$S+I+R=1 \Rightarrow R=1-S-I$$

$$\dot{S} = -\beta SI + \alpha(1-S-I)$$

$$\dot{I} = \beta SI - \gamma I$$

$$J=\begin{bmatrix} \frac{dF}{dS} & \frac{dF}{dI} \\ \frac{dG}{dS} & \frac{dG}{dI}\end{bmatrix}$$

$$J = \begin{bmatrix}-\beta I^* - \alpha & -\beta S^*-\alpha \\ \beta I^* & \beta S^* - \gamma\end{bmatrix}$$

Disease Free Equilibria:
DFE: $I^* = 0$, $S^* = 1$

$det(J_{DFE} - \lambda I) = 0$, Where I = Identity Matrix:

Example $\rightarrow \begin{bmatrix} 0 & 1 \\ 1 & 0\end{bmatrix}=I^2$

$$J_{DFE} = \begin{bmatrix}-\alpha & -\beta-\alpha \\ 0 & \beta-\gamma\end{bmatrix}$$

$$det(\begin{bmatrix}-\alpha & -\beta-\alpha \\ 0 & \beta-\gamma\end{bmatrix}-\lambda\begin{bmatrix} 0 & 1 \\ 1 & 0\end{bmatrix})$$

Distribute Lambda:
$$det(\begin{bmatrix}-\alpha & -\beta-\alpha \\ 0 & \beta-\gamma\end{bmatrix}+\begin{bmatrix}-\lambda & 0 \\ 0 & -\lambda\end{bmatrix}) =$$

$$det(\begin{bmatrix}-\alpha-\lambda & -\beta-\alpha \\ 0 & \beta-\gamma-\lambda\end{bmatrix})$$

$$det(\begin{bmatrix} A & B \\ C & D\end{bmatrix}) = AD-BC$$

So:
$$det(\begin{bmatrix}-\alpha-\lambda & -\beta-\alpha \\ 0 & \beta-\gamma-\lambda\end{bmatrix}) = -(\alpha+\lambda)(\beta-\gamma-\lambda)-0=0$$

Set Equal to 0:
$$-(\alpha+\lambda)=0\\(\beta-\gamma-\lambda)=0$$

Eigenvalues are:
$$\lambda = -\alpha\\ \lambda= \beta-\gamma$$

An equilibrium is stable if all the eigenvalues of the Jacobian matrix evaluated at the equilibrium have negative real parts. If any eigenvalue is positive, then the equilibrium is unstable. If some eigenvalues are zero and the rest are negative, then stability is inconclusive.

$$\lambda_1 = -\alpha < 0$$

$$\lambda_2 = \beta - \gamma < 0 \Rightarrow \beta<\gamma \Rightarrow \frac{\beta}{\gamma} = R_0 < 1$$

DFE is stable if $\frac{\beta}{\gamma} = R_0 < 1$

Endemic Equilibrium
$S^*=\frac{\gamma}{\beta}=1/R_0$ only makes sense if $R_0>1$. Thus if this equilibrium exists the DFE is unstable.

$$I^*=\frac{\alpha (1 - \frac{\gamma}{\beta})}{\gamma + \alpha}$$

$$\dot{S} = -\beta SI + \alpha(1-S-I)$$

$$\dot{I} = \beta SI - \gamma I$$

$$J = \begin{bmatrix}-\beta I - \alpha & -\beta S-\alpha \\ \beta I & \beta S - \gamma\end{bmatrix}$$

$$J = \begin{bmatrix}-\beta I^* - \alpha & -\gamma-\alpha \\ \beta I & 0\end{bmatrix}$$

$$det(J-\lambda I) = 0 \\ det(\lambda I - J) = 0$$

$$det(\begin{bmatrix}-\beta I* - \alpha -\lambda & -\gamma-\alpha \\ \beta I & -\lambda\end{bmatrix})$$

$$(\beta I^* + \alpha + \lambda)\lambda + \beta I^*(\gamma+\alpha) = 0$$

Characteristic Equation:
$$\lambda^2 + (\beta I^* + \alpha)\lambda + \beta I^*(\gamma+\alpha) = 0$$

Where $a=\lambda^2, b=(\beta I^* + \alpha), c=\beta I^*(\gamma+\alpha)$

$$\lambda^2 + \alpha \left[ \frac{1 - \frac{1}{R_0}}{R_0 + \frac{\alpha}{\beta}} + 1 \right] + \alpha\beta(1-\frac{1}{R_0})=0$$

Subsitute a, b, c into quadratic equation:

$$\lambda = \frac{-\alpha \left[ \frac{1 - \frac{1}{R_0}}{R_0 + \frac{\alpha}{\beta}} + 1 \right] \pm \sqrt{(\beta I^* + \alpha)^2 - 4\beta I(\gamma+\alpha)}}{2}$$

Where $-\alpha \left[ \frac{1 - \frac{1}{R_0}}{R_0 + \frac{\alpha}{\beta}} + 1 \right]$ is negative due to the signage

$$(\beta I^* + \alpha)^2 - 4\beta I(\gamma+\alpha) = \beta^2 (I^*)^2 + \alpha^2 + 2\beta(I^*)^2 - 4\beta I \alpha - 4\beta I \gamma$$

$$\lambda = \frac{-(\beta I^*+\alpha) \pm \sqrt{(\beta I^* + \alpha)^2 - 4\beta I(\gamma+\alpha)}}{2}$$

$\lambda = \frac{-b}{2}$ $\pm$ Complex Number, where $\frac{-b}{2}$ is a real part.

$$\lambda=a \pm bi$$
$$\lambda_1 = a + bi$$
$$\lambda_2=a-bi$$

$Z=a+bi$ where $i=\sqrt{-1}$ and $a$ and $b$ are real;
$Re(Z)=$ $a$ real part of $Z$, and $Im(Z)=$ $b$, imaginary number.

$$b^2>b^2-4c>0$$
$$\lambda_1=\frac{{-b} + \sqrt{(b^2 - 4c)^2}}{2}<0$$

$\lambda_2=\frac{{-b} - \sqrt{(b^2 - 4c)}}{2}$ where $b^2>b^2 - 4c$, so

$<\frac{{-b} - \sqrt{b^2}}{2}=0$

Notice $\pm$, only focus on $+$ and drop $- 4\beta I(\gamma+\alpha)$ due to complexity:

$$<\frac{-(\beta I^*+\alpha) \pm \sqrt{(\beta I^* + \alpha)^2}}{2}=\frac{-(\beta I^*+\alpha)+{(\beta I^* + \alpha)}}{2}=0$$

Both eigenvalues are negative and it is stable.

Routh - Hurwitz Criteria
$$\sum{i}c_ix^i=c_2\lambda^2 + c_1\lambda + c_0$$

Where, $c_i>0$

Quadratic Characteristic Equation:

- Minimum of the characterisitic equation:

$$2\lambda + \beta I + \alpha = 0$$

$$\lambda = \frac{-\beta I + \alpha}{2}$$

$$\frac{(\beta I + \alpha)^2}{4}-\frac{(\beta I + \alpha)^2}{2}+\beta I(\gamma+\alpha)=$$

$$1/4[(\beta I+\alpha)^2-2(\beta I+\alpha)^2+4(\beta I(\gamma+\alpha))]=$$

$$1/4[-(\beta I+\alpha)^2+4(\beta I(\gamma+\alpha))]=$$

$$1/4[-\beta^2 I^2 - 2\beta I \alpha -\alpha^2 + 4\beta I \gamma + 4 \beta I \alpha]=$$

$$1/4[-\beta^2 I^2 + 2\beta I \alpha -\alpha^2 + 4\beta I \gamma]>0$$

Descartes' Rule of Signs:

$$c_2\lambda^2 + c_1\lambda + c_0 = 0$$

0 sign changes from term to term

- All terms are positive

So there are either 0 positive roots or 2 positive roots

$$c_2(-\lambda)^2+c_1(-\lambda)+c_0=0$$

$$c_2\lambda^2-c_1\lambda+c_0=0$$

2 sign changes from term to term

- First and last term are positive, while middle term is negative
- From first to second term, $+$ to $-$, first sign change
- From second to third term, $-$ to $+$, second sign change

So there are either 2 negative roots or zero negaive roots

Cases where there is one sign change:

Example:

$(-) \rightarrow (+) (+)$$\cdots$$\lambda \rightarrow$ 1 Positive Root

$(-) (-) \rightarrow (+)$$\cdots$$-\lambda \rightarrow$ 1 Negative Root

For $S(t)$, $S=\frac{\gamma}{\beta}$

DFE: $I^*=0$, $S*=1$

$$S(t) =\left[\begin{aligned}&\dot{S} = -\beta SI + \alpha I\\&\dot{S}=(-\beta S \gamma)(1-S)\\&\dot{I} = \beta SI - \gamma I\\&J = -\beta(1-S) - (-\beta S + \gamma) = -\beta + \beta S + \beta S - \gamma = 2\beta S - \beta - \gamma\\&J_{DFE} = -\beta(1-1) - (-\beta + \gamma) = \beta - \gamma < 0 \rightarrow \beta < \gamma = R_0 < 1 \\&J_{EE} = 2\beta \left(\frac{\gamma}{\beta}\right) - \beta - \gamma = 2\gamma - \beta - \gamma = \gamma - \beta < 0 \rightarrow 1 < R_0\end{aligned} \right]$$
